Core/Term/Substitution.lean
@@ -28,29 +28,29 @@ instance : Coe (Subst.Action Term) Term where
   coe := Term.from_action
 
 @[simp]
-def Term.rmap (lf : Endo Ren) (r : Ren) : Term -> Term
+def Term.rmap (r : Ren) : Term -> Term
 | #x => #(r x)
 | g#x => g#x
 | ctor0 c => ctor0 c
-| ctor1 c t => ctor1 c (rmap lf r t)
-| ctor2 c t1 t2 => ctor2 c (rmap lf r t1) (rmap lf r t2)
-| tbind v A t => tbind v A (rmap lf r t)
-| lam A t => lam A (rmap lf (lf r) t)
-| guard t1 t2 t3 => guard (rmap lf r t1) (rmap lf r t2) (rmap lf r t3)
-| .match t1 t2 t3 t4 => .match (rmap lf r t1) (λ i => rmap lf r (t2 i)) (λ i => rmap lf r (t3 i)) (rmap lf r t4)
+| ctor1 c t => ctor1 c (rmap r t)
+| ctor2 c t1 t2 => ctor2 c (rmap r t1) (rmap r t2)
+| tbind v A t => tbind v A (rmap r t)
+| lam A t => lam A (rmap r.lift t)
+| guard t1 t2 t3 => guard (rmap r t1) (rmap r t2) (rmap r t3)
+| .match t1 t2 t3 t4 => .match (rmap r t1) (λ i => rmap r (t2 i)) (λ i => rmap r (t3 i)) (rmap r t4)
 
 instance : RenMap Term where
   rmap := Term.rmap
 
 @[simp]
-def Ctor0Variant.rmap (_ : Endo Ren) (_ : Ren) : Ctor0Variant -> Ctor0Variant
+def Ctor0Variant.rmap (_ : Ren) : Ctor0Variant -> Ctor0Variant
 | c => c
 
 instance : RenMap Ctor0Variant where
   rmap := Ctor0Variant.rmap
 
 @[simp]
-def Ctor0Variant.smap (_ : Endo (Subst Ctor0Variant)) (_ : Subst Ctor0Variant) : Ctor0Variant -> Ctor0Variant
+def Ctor0Variant.smap (_ : Subst Ctor0Variant) : Ctor0Variant -> Ctor0Variant
 | c => c
 
 instance : SubstMap Ctor0Variant Ctor0Variant where
@@ -58,7 +58,7 @@ instance : SubstMap Ctor0Variant Ctor0Variant where
 
 @[simp]
 theorem Ctor0Variant.subst_ {c : Ctor0Variant} : c[σ:Ctor0Variant] = c := by
-  simp [Subst.apply, SubstMap.smap]
+  simp [SubstMap.smap]
 
 instance : SubstMapId Ctor0Variant Ctor0Variant where
   apply_id := by simp
@@ -67,7 +67,7 @@ instance : SubstMapCompose Ctor0Variant Ctor0Variant where
   apply_compose := by simp
 
 @[simp]
-def Ctor0Variant.Ty.smap (_ : Endo (Subst Ty)) (σ : Subst Ty) : Ctor0Variant -> Ctor0Variant
+def Ctor0Variant.Ty.smap (σ : Subst Ty) : Ctor0Variant -> Ctor0Variant
 | zero => zero
 | refl A => refl A[σ:_]
 
@@ -76,11 +76,11 @@ instance : SubstMap Ctor0Variant Ty where
 
 @[simp]
 theorem Ctor0Variant.subst_zero : zero[σ:Ty] = zero := by
-  simp [Subst.apply, SubstMap.smap]
+  simp [SubstMap.smap]
 
 @[simp]
 theorem Ctor0Variant.subst_refl : (refl A)[σ:Ty] = refl A[σ:_] := by
-  simp [Subst.apply, SubstMap.smap]
+  simp [SubstMap.smap]
 
 instance : SubstMapId Ctor0Variant Ty where
   apply_id := by intro t; cases t <;> simp
@@ -92,14 +92,14 @@ instance : SubstMapHetCompose Ctor0Variant Ty where
   apply_hcompose := by simp
 
 @[simp]
-def Ctor1Variant.rmap (_ : Endo Ren) (_ : Ren) : Ctor1Variant -> Ctor1Variant
+def Ctor1Variant.rmap (_ : Ren) : Ctor1Variant -> Ctor1Variant
 | c => c
 
 instance : RenMap Ctor1Variant where
   rmap := Ctor1Variant.rmap
 
 @[simp]
-def Ctor1Variant.smap (_ : Endo (Subst Ctor1Variant)) (_ : Subst Ctor1Variant) : Ctor1Variant -> Ctor1Variant
+def Ctor1Variant.smap (_ : Subst Ctor1Variant) : Ctor1Variant -> Ctor1Variant
 | c => c
 
 instance : SubstMap Ctor1Variant Ctor1Variant where
@@ -107,7 +107,7 @@ instance : SubstMap Ctor1Variant Ctor1Variant where
 
 @[simp]
 theorem Ctor1Variant.subst_ {c : Ctor1Variant} : c[σ:Ctor1Variant] = c := by
-  simp [Subst.apply, SubstMap.smap]
+  simp [SubstMap.smap]
 
 instance : SubstMapId Ctor1Variant Ctor1Variant where
   apply_id := by simp
@@ -116,7 +116,7 @@ instance : SubstMapCompose Ctor1Variant Ctor1Variant where
   apply_compose := by simp
 
 @[simp]
-def Ctor1Variant.Ty.smap (_ : Endo (Subst Ty)) (σ : Subst Ty) : Ctor1Variant -> Ctor1Variant
+def Ctor1Variant.Ty.smap (σ : Subst Ty) : Ctor1Variant -> Ctor1Variant
 | sym => sym
 | fst => fst
 | snd => snd
@@ -127,19 +127,19 @@ instance : SubstMap Ctor1Variant Ty where
 
 @[simp]
 theorem Ctor1Variant.subst_sym : sym[σ:Ty] = sym := by
-  simp [Subst.apply, SubstMap.smap]
+  simp [SubstMap.smap]
 
 @[simp]
 theorem Ctor1Variant.subst_fst : (fst)[σ:Ty] = fst := by
-  simp [Subst.apply, SubstMap.smap]
+  simp [SubstMap.smap]
 
 @[simp]
 theorem Ctor1Variant.subst_snd : (snd)[σ:Ty] = snd := by
-  simp [Subst.apply, SubstMap.smap]
+  simp [SubstMap.smap]
 
 @[simp]
 theorem Ctor1Variant.subst_appt : (appt a)[σ:Ty] = appt a[σ:_] := by
-  simp [Subst.apply, SubstMap.smap]
+  simp [SubstMap.smap]
 
 instance : SubstMapId Ctor1Variant Ty where
   apply_id := by intro t; cases t <;> simp
@@ -151,14 +151,14 @@ instance : SubstMapHetCompose Ctor1Variant Ty where
   apply_hcompose := by simp
 
 @[simp]
-def Ctor2Variant.rmap (_ : Endo Ren) (_ : Ren) : Ctor2Variant -> Ctor2Variant
+def Ctor2Variant.rmap (_ : Ren) : Ctor2Variant -> Ctor2Variant
 | c => c
 
 instance : RenMap Ctor2Variant where
   rmap := Ctor2Variant.rmap
 
 @[simp]
-def Ctor2Variant.smap (_ : Endo (Subst Ctor2Variant)) (_ : Subst Ctor2Variant) : Ctor2Variant -> Ctor2Variant
+def Ctor2Variant.smap (_ : Subst Ctor2Variant) : Ctor2Variant -> Ctor2Variant
 | c => c
 
 instance : SubstMap Ctor2Variant Ctor2Variant where
@@ -166,7 +166,7 @@ instance : SubstMap Ctor2Variant Ctor2Variant where
 
 @[simp]
 theorem Ctor2Variant.subst_ {c : Ctor2Variant} : c[σ:Ctor2Variant] = c := by
-  simp [Subst.apply, SubstMap.smap]
+  simp [SubstMap.smap]
 
 instance : SubstMapId Ctor2Variant Ctor2Variant where
   apply_id := by simp
@@ -175,7 +175,7 @@ instance : SubstMapCompose Ctor2Variant Ctor2Variant where
   apply_compose := by simp
 
 @[simp]
-def Ctor2Variant.Ty.smap (_ : Endo (Subst Ty)) (_ : Subst Ty) : Ctor2Variant -> Ctor2Variant
+def Ctor2Variant.Ty.smap (_ : Subst Ty) : Ctor2Variant -> Ctor2Variant
 | c => c
 
 instance : SubstMap Ctor2Variant Ty where
@@ -183,7 +183,7 @@ instance : SubstMap Ctor2Variant Ty where
 
 @[simp]
 theorem Ctor2Variant.Ty.subst_ {c : Ctor2Variant} : c[σ:Ty] = c := by
-  simp [Subst.apply, SubstMap.smap]
+  simp [SubstMap.smap]
 
 instance : SubstMapId Ctor2Variant Ty where
   apply_id := by intro t; cases t <;> simp
@@ -195,72 +195,72 @@ instance : SubstMapHetCompose Ctor2Variant Ty where
   apply_hcompose := by simp
 
 @[simp]
-def Term.Ty.smap (lf : Endo (Subst Ty)) (σ : Subst Ty) : Term -> Term
+def Term.Ty.smap (σ : Subst Ty) : Term -> Term
 | #x => #x
 | g#x => g#x
 | ctor0 c => ctor0 c[σ:Ty]
-| ctor1 c t => ctor1 c[σ:Ty] (smap lf σ t)
-| ctor2 c t1 t2 => ctor2 c[σ:Ty] (smap lf σ t1) (smap lf σ t2)
-| tbind v A t => tbind v A (smap lf (lf σ) t)
-| lam A t => lam A[σ:_] (smap lf σ t)
-| guard t1 t2 t3 => guard (smap lf σ t1) (smap lf σ t2) (smap lf σ t3)
-| .match t1 t2 t3 t4  => .match (smap lf σ t1) (λ i => smap lf σ (t2 i)) (λ i => smap lf σ (t3 i)) (smap lf σ t4)
+| ctor1 c t => ctor1 c[σ:Ty] (smap σ t)
+| ctor2 c t1 t2 => ctor2 c[σ:Ty] (smap σ t1) (smap σ t2)
+| tbind v A t => tbind v A (smap σ.lift t)
+| lam A t => lam A[σ:_] (smap σ t)
+| guard t1 t2 t3 => guard (smap σ t1) (smap σ t2) (smap σ t3)
+| .match t1 t2 t3 t4  => .match (smap σ t1) (λ i => smap σ (t2 i)) (λ i => smap σ (t3 i)) (smap σ t4)
 
 instance : SubstMap Term Ty where
   smap := Term.Ty.smap
 
 @[simp]
-def Term.smap (lf : Endo (Subst Term)) (σ : Subst Term) : Term -> Term
+def Term.smap (σ : Subst Term) : Term -> Term
 | #x => σ x
 | g#x => g#x
 | ctor0 c => ctor0 c
-| ctor1 c t => ctor1 c (smap lf σ t)
-| ctor2 c t1 t2 => ctor2 c (smap lf σ t1) (smap lf σ t2)
-| tbind v A t => tbind v A (smap lf (σ ◾ +1@Ty) t)
-| lam A t => lam A (smap lf (lf σ) t)
-| guard t1 t2 t3 => guard (smap lf σ t1) (smap lf σ t2) (smap lf σ t3)
-| .match t1 t2 t3 t4 => .match (smap lf σ t1) (λ i => smap lf σ (t2 i)) (λ i => smap lf σ (t3 i)) (smap lf σ t4)
+| ctor1 c t => ctor1 c (smap σ t)
+| ctor2 c t1 t2 => ctor2 c (smap σ t1) (smap σ t2)
+| tbind v A t => tbind v A (smap (σ ◾ +1@Ty) t)
+| lam A t => lam A (smap σ.lift t)
+| guard t1 t2 t3 => guard (smap σ t1) (smap σ t2) (smap σ t3)
+| .match t1 t2 t3 t4 => .match (smap σ t1) (λ i => smap σ (t2 i)) (λ i => smap σ (t3 i)) (smap σ t4)
 
 instance : SubstMap Term Term where
   smap := Term.smap
 
 @[simp]
 theorem Term.subst_var : (#x)[σ:Term] = σ x := by
-  unfold Subst.apply; simp [SubstMap.smap]
+  simp [SubstMap.smap]
 
 @[simp]
 theorem Term.subst_global : (g#x)[σ:Term] = g#x := by
-  unfold Subst.apply; simp [SubstMap.smap]
+  simp [SubstMap.smap]
 
 @[simp]
 theorem Term.subst_ctor0 : (ctor0 v)[σ:Term] = ctor0 v := by
-  simp [Subst.apply, SubstMap.smap]
+  simp [SubstMap.smap]
 
 @[simp]
 theorem Term.subst_ctor1 : (ctor1 v t)[σ:Term] = ctor1 v t[σ:_] := by
-  simp [Subst.apply, SubstMap.smap]
+  simp [SubstMap.smap]
 
 @[simp]
 theorem Term.subst_ctor2 : (ctor2 v t1 t2)[σ:Term] = ctor2 v t1[σ:_] t2[σ:_] := by
-  simp [Subst.apply, SubstMap.smap]
+  simp [SubstMap.smap]
 
 @[simp]
 theorem Term.subst_tbind : (tbind v A t)[σ:Term] = tbind v A t[σ ◾ +1@Ty:_] := by
-  simp [Subst.apply, SubstMap.smap]
+  simp [SubstMap.smap]
 
 @[simp]
 theorem Term.subst_lam : (lam A t)[σ:Term] = lam A t[σ.lift:_] := by
-  simp [Subst.apply, SubstMap.smap]
+  simp [SubstMap.smap]
 
 @[simp]
 theorem Term.subst_guard : (guard t1 t2 t3)[σ:Term] = guard t1[σ:_] t2[σ:_] t3[σ:_] := by
-  simp [Subst.apply, SubstMap.smap]
+  simp [SubstMap.smap]
 
 @[simp]
 theorem Term.subst_match
   : (match! t1 t2 t3 t4)[σ:Term] = match! t1[σ:_] (λ i => (t2 i)[σ:_]) (λ i => (t3 i)[σ:_]) (t4[σ:_])
 := by
-  simp [Subst.apply, SubstMap.smap]
+  simp [SubstMap.smap]
 
 @[simp]
 theorem Term.from_action_compose {x} {σ τ : Subst Term}
@@ -272,41 +272,41 @@ theorem Term.from_action_compose {x} {σ τ : Subst Term}
 
 @[simp]
 theorem Term.Ty.subst_var : (#x)[σ:Ty] = #x := by
-  unfold Subst.apply; simp [SubstMap.smap]
+  simp [SubstMap.smap]
 
 @[simp]
 theorem Term.Ty.subst_global : (g#x)[σ:Ty] = g#x := by
-  unfold Subst.apply; simp [SubstMap.smap]
+  simp [SubstMap.smap]
 
 @[simp]
 theorem Term.Ty.subst_ctor0 : (ctor0 c)[σ:Ty] = ctor0 c[σ:_] := by
-  simp [Subst.apply, SubstMap.smap]
+  simp [SubstMap.smap]
 
 @[simp]
 theorem Term.Ty.subst_ctor1 : (ctor1 c t)[σ:Ty] = ctor1 c[σ:_] t[σ:_] := by
-  simp [Subst.apply, SubstMap.smap]
+  simp [SubstMap.smap]
 
 @[simp]
 theorem Term.Ty.subst_ctor2 : (ctor2 c t1 t2)[σ:Ty] = ctor2 c[σ:_] t1[σ:_] t2[σ:_] := by
-  simp [Subst.apply, SubstMap.smap]
+  simp [SubstMap.smap]
 
 @[simp]
 theorem Term.Ty.subst_tbind : (tbind b A t)[σ:Ty] = tbind b A t[σ.lift:_] := by
-  simp [Subst.apply, SubstMap.smap]
+  simp [SubstMap.smap]
 
 @[simp]
 theorem Term.Ty.subst_lam : (lam A t)[σ:Ty] = lam A[σ:_] t[σ:_] := by
-  simp [Subst.apply, SubstMap.smap]
+  simp [SubstMap.smap]
 
 @[simp]
 theorem Term.Ty.subst_guard : (guard t1 t2 t3)[σ:Ty] = guard t1[σ:_] t2[σ:_] t3[σ:_] := by
-  simp [Subst.apply, SubstMap.smap]
+  simp [SubstMap.smap]
 
 @[simp]
 theorem Term.Ty.subst_match
   : (match! t1 ps t2 t3)[σ:Ty] = match! t1[σ:_] (λ i => (ps i)[σ:_]) (λ i => (t2 i)[σ:_]) t3[σ:_]
 := by
-  simp [Subst.apply, SubstMap.smap]
+  simp [SubstMap.smap]
 
 theorem Term.Ty.apply_id {t : Term} : t[+0:Ty] = t := by
   induction t
@@ -324,8 +324,8 @@ theorem Term.hcompose_var {σ : Subst Term} {τ : Subst Ty}
   cases z <;> simp
 
 theorem Term.apply_stable (r : Ren) (σ : Subst Term)
-  : r.to = σ -> Ren.apply (T := Term) r = Subst.apply σ
-:= by subst_solve_stable Term, r, σ
+  : r = σ -> rmap r = smap σ
+:= by subst_solve_stable r, σ
 
 
 instance : SubstMapStable Term where
@@ -338,7 +338,7 @@ theorem Term.apply_ren_commute {s : Term} (r : Ren) (τ : Subst Ty)
   all_goals try simp [*]
   case lam A t ih =>
     replace ih := ih r.lift
-    rw [Ren.to_lift (S := Term)] at ih; simp at ih
+    rw [Ren.to_lift] at ih; simp at ih
     apply ih
 
 instance : SubstMapRenCommute Term Ty where
@@ -357,7 +357,7 @@ theorem Term.apply_hcompose {s : Term} {σ : Subst Term} {τ : Subst Ty}
 instance : SubstMapHetCompose Term Ty where
   apply_hcompose := Term.apply_hcompose
 
-theorem Term.apply_id {t : Term} : t[+0] = t := by subst_solve_id Term, Ty, t
+theorem Term.apply_id {t : Term} : t[+0] = t := by induction t <;> (simp at *; try simp [*])
 
 instance : SubstMapId Term Term where
   apply_id := Term.apply_id
